LeanYjs/ItemSet.lean
@@ -6,12 +6,10 @@ import Mathlib.Tactic.Set
 
 variable (A : Type) [BEq A]
 
-structure IsClosedItemPredicate (P : YjsPtr A -> Prop) : Prop where
+def ItemSet := Set (YjsPtr A)
+
+structure IsClosedItemSet {A} (P : YjsPtr A -> Prop) : Prop where
   baseFirst : P YjsPtr.first
   baseLast : P YjsPtr.last
   closedLeft : (∀ (o : YjsPtr A) r id c, P (YjsItem.item o r id c) -> P o)
   closedRight : (∀ o (r : YjsPtr A) id c, P (YjsItem.item o r id c) -> P r)
-
-def ClosedPredicate := { P : YjsPtr A -> Prop // IsClosedItemPredicate A P }
-
-def ItemSet (P : ClosedPredicate A) := { i : YjsPtr A // P.val i }
