LeanYjs/OrderCases.lean
@@ -5,7 +5,7 @@ import LeanYjs.ItemOrder
 import LeanYjs.ItemSet
 import LeanYjs.ItemSetInvariant
 
-def yjsLtConcurrent {A : Type} {P : ClosedPredicate A} (x y : YjsItem A) : Prop :=
+def yjsLtConcurrent {A : Type} {P : ItemSet A} (x y : YjsItem A) : Prop :=
   ∃ h1 h2 h3 h4,
     YjsLt P h1 x.origin y ∧
     YjsLt P h2 y x.rightOrigin ∧
